Forward simulation for the 4 encoding passes (Str-, Sym-, Reloc-, Shstr-table)
x86/RelocProgSemantics3.v
x86/TablesEncodeproof.v

encode/Encode.v
@@ -49,3 +49,74 @@ Proof.
   unfold decode_int16, encode_int16.
   rewrite decode_encode_int. reflexivity.
 Qed.
+
+Require Import Coqlib Errors List.
+Local Open Scope error_monad_scope.
+(* Local Open Scope hex_scope. *)
+(* Local Open Scope bits_scope. *)
+
+
+
+Fixpoint take_drop {A} n (l: list A) : res (list A * list A) :=
+  match n, l with
+  | O, l => OK ([], l)
+  | S n, a::r =>
+    do (a1,b1) <- take_drop n r ;
+    OK (a::a1, b1)
+  | S n, [] => Error (msg "take_drop: list too short")
+  end.
+
+Lemma take_drop_encode_int sz x l:
+  take_drop sz (encode_int sz x ++ l) = OK (encode_int sz x, l).
+Proof.
+  generalize (encode_int_length sz x).
+  generalize (encode_int sz x).
+  induction sz; simpl; intros; eauto.
+  - destruct l0; simpl in *; try congruence.
+  - destruct l0; simpl in *; try congruence.
+    rewrite IHsz. simpl. auto. congruence.
+Qed.
+
+Lemma take_drop_cons {A} x (l: list A):
+  take_drop 1 (x :: l) = OK ([x], l).
+Proof.
+  reflexivity.
+Qed.
+
+
+Lemma take_drop_length {A} sz (l: list A):
+  length l = sz ->
+  take_drop sz l = OK (l, []).
+Proof.
+  revert l.
+  induction sz; simpl; intros; eauto.
+  - destruct l; simpl in *; try congruence.
+  - destruct l; simpl in *; try congruence.
+    rewrite IHsz. simpl. auto. congruence.
+Qed.
+
+
+Lemma take_drop_length_app {A} sz (l1 l2: list A):
+  length l1 = sz ->
+  take_drop sz (l1 ++ l2) = OK (l1, l2).
+Proof.
+  revert l1 l2.
+  induction sz; simpl; intros; eauto.
+  - destruct l1; simpl in *; try congruence.
+  - destruct l1; simpl in *; try congruence.
+    rewrite IHsz. simpl. auto. congruence.
+Qed.
+
+
+Lemma take_drop_length_2 :
+  forall {A} z (l: list A) l1 l2,
+    (z > 0)%nat ->
+    take_drop z l = OK (l1, l2) ->
+    (length l2 < length l)%nat.
+Proof.
+  induction z; simpl; intros; eauto. omega.
+  destr_in H0. monadInv H0.
+  destruct z.  simpl in *. inv EQ.  omega.
+  apply IHz in EQ. simpl. omega. omega.
+Qed.
+
