x86/StrtableEncode.v
@@ -28,22 +28,24 @@ Definition acc_symbol_strings id r :=
     Error [MSG "Cannot find the string of the symbol "; CTX id]
   | Some pos_nums =>
     let bytes := map (fun p => Byte.repr (Zpos p)) pos_nums in
-    OK ((id, HB["00"] :: bytes) :: idbytes)
+    OK ((id, bytes ++ [HB["00"]]) :: idbytes)
   end.
 
 Definition acc_strmap r (idb: ident * list byte) := 
-  let '(map,sz) := r in
+  let '(map,next) := r in
   let '(id, bytes) := idb in
-  let map' := PTree.set id (sz+1) map in
-  let sz'  := sz + Z.of_nat(length bytes) in
-  (map', sz').
+  let map' := PTree.set id next map in
+  let next'  := next + Z.of_nat(length bytes) + 1 in
+  (map', next').
 
 Definition get_strings_map_bytes (symbols: list ident) : res (PTree.t Z * list byte) :=
   do idbytes <-
      fold_right acc_symbol_strings (OK []) symbols;
-  let '(strmap, _) := fold_left acc_strmap idbytes (PTree.empty Z, 0) in
+  let '(strmap, maxofs) := fold_left acc_strmap idbytes (PTree.empty Z, 1) in
   let sbytes := fold_right (fun '(id,bytes) acc => bytes ++ acc) [] idbytes in
-  OK (strmap, sbytes ++ [HB["00"]]).
+  if zlt maxofs Int.max_unsigned then
+    OK (strmap, sbytes)
+  else Error (msg "Too many strings").
                              
 Definition create_strtab_section (strs: list byte) := sec_bytes strs.
 
@@ -66,7 +68,7 @@ Definition transf_program (p:program) : res program :=
         prog_sectable := p.(prog_sectable) ++ [strsec];
         prog_strtable := strmap;
         prog_symbtable := p.(prog_symbtable);
-        prog_reloctables := p.(prog_reloctables);
+        prog_reloctables := prog_reloctables p;
         prog_senv := p.(prog_senv);
      |} in
   let len := (length (prog_sectable p')) in
@@ -74,3 +76,82 @@ Definition transf_program (p:program) : res program :=
     OK p'
   else
     Error [MSG "In Strtablegen: number of sections is incorrect (not 4): "; POS (Pos.of_nat len)].
+
+Record valid_strtable_thr (strtab: strtable) o: Prop :=
+  {
+    nodupstr: forall i j x y,
+      strtab ! i = Some x -> strtab ! j = Some y -> i <> j ->
+      x <> y;
+    thr: forall i x, strtab ! i = Some x -> x < o;
+    table_range: forall i x, strtab ! i = Some x -> 0 <= x < two_p 32;
+    strtab_no_0:
+      forall i : positive, strtab ! i = Some 0 -> False;
+  }.
+
+Lemma acc_strmap_fold_lt:
+  forall x t z t0 z1,
+    fold_left acc_strmap x (t,z) = (t0, z1) ->
+    z <= z1.
+Proof.
+  induction x; simpl; intros; eauto. inv H. omega.
+  destr_in H.
+  apply IHx in H. omega.
+Qed.
+
+Definition valid_strtable tab :=
+  exists o, valid_strtable_thr tab o /\ o < Int.max_unsigned.
+
+Lemma transf_program_valid_strtable:
+  forall pi p (TF: transf_program pi = OK p),
+    valid_strtable (prog_strtable p).
+Proof.
+  intros pi p TF.
+  unfold valid_strtable.
+  unfold transf_program in TF.
+  monadInv TF.
+  repeat destr_in EQ0. simpl in *.
+  apply beq_nat_true in Heqb.
+  destruct (prog_sectable pi); simpl in *; try congruence.
+  destruct s0; simpl in *; try congruence.
+  destruct s1; simpl in *; try congruence.
+  destruct s2; simpl in *; try congruence.
+  2: destruct s3; simpl in *; try congruence.
+  unfold get_strings_map_bytes in EQ.
+  monadInv EQ. repeat destr_in EQ1.
+  exists z; split; auto.
+  revert z Heqp l0.
+  assert (valid_strtable_thr (PTree.empty Z) 1 /\ 0 < 1).
+  {
+    split.
+    constructor; setoid_rewrite PTree.gempty; congruence.
+    omega.
+  }
+  generalize t.
+  destruct H as (VALID & POS).
+  revert VALID POS.
+  generalize (PTree.empty Z) 1.
+  clear.
+  induction x; simpl.
+  - intros; eauto. inv Heqp. eauto.
+  - intros t z VALID POS t0 z1 FOLD LT.
+    destr_in FOLD.
+    eapply IHx in FOLD. auto.
+    constructor; repeat setoid_rewrite PTree.gsspec.
+    + intros i0 j x0 y. repeat destr.
+      * intros A; inv A. inv VALID. intro B; apply thr0 in B. omega.
+      * subst. intro B. inv VALID. apply thr0 in B. intro A; inv A. omega.
+      * inv VALID; eauto.
+    + intros i0 x0. destr.
+      * intro A; inv A.
+        omega.
+      * inv VALID. intro A; apply thr0 in A. omega.
+    + intros i0 x0 EQ. destr_in EQ.
+      * inv EQ.
+        apply acc_strmap_fold_lt in FOLD. change (two_p 32) with (Int.max_unsigned + 1).
+        omega.
+      * inv VALID; eauto.
+    + intros i0 EQ. destr_in EQ. inv EQ.
+      omega. inv VALID; eauto.
+    + omega.
+    + auto.
+Qed.
