x86/RelocProgSemantics3.v
@@ -1,0 +1,65 @@
+(* *******************  *)
+(* Author: Pierre Wilke  *)
+(* Date:  Jan 7, 2020  *)
+(* *******************  *)
+
+(** * The semantics of relocatable program after string table, section header string
+table and symbol table encoding *)
+
+
+Require Import Coqlib Maps AST Integers Values.
+Require Import Events Floats Memory Smallstep.
+Require Import Asm RelocProgram RawAsm Globalenvs.
+Require Import Stacklayout Conventions EraseArgs.
+Require Import Linking SeqTable Errors.
+Require Import SymbtableDecode StrtableDecode ShstrtableDecode ReloctablesDecode.
+Require RelocProgSemantics2.
+
+Local Open Scope error_monad_scope.
+
+
+Section WITHEXTERNALCALLS.
+Context `{external_calls_prf: ExternalCalls}.
+
+Definition decode_tables (p:program) : res program :=
+  do p <- ShstrtableDecode.transf_program_inv p;
+    do p <- ReloctablesDecode.transf_program_inv p;
+    do p <- SymbtableDecode.transf_program_inv p;
+    do p <- StrtableDecode.transf_program_inv p; OK p.
+
+Inductive initial_state (prog: program) (rs: regset) (s: state): Prop :=
+| initial_state_intro: forall prog',
+    decode_tables prog = OK prog' ->
+    RelocProgSemantics2.initial_state prog' rs s ->
+    initial_state prog rs s.
+
+Definition semantics (p: program) (rs: regset) :=
+  Semantics_gen RelocProgSemantics1.step
+                (initial_state p rs) RelocProgSemantics1.final_state
+                (RelocProgSemantics1.globalenv p)
+                (RelocProgSemantics1.genv_senv (RelocProgSemantics1.globalenv p)).
+
+
+(** Determinacy of the semantics. *)
+
+Lemma semantics_determinate: forall p rs, determinate (semantics p rs).
+Proof.
+  intros.
+  constructor; simpl; auto.
+  - intros; eapply (sd_determ (RelocProgSemantics2.semantics_determinate p rs)); eauto.
+  - intros; eapply (sd_traces (RelocProgSemantics2.semantics_determinate p rs)); eauto.
+  - intros s1 s2 H H0. inv H; inv H0.
+    assert (prog' = prog'0) by congruence. subst.
+    intros; eapply (sd_initial_determ (RelocProgSemantics2.semantics_determinate prog'0 rs)); eauto.
+  - intros; eapply (sd_final_nostep (RelocProgSemantics2.semantics_determinate p rs)); eauto.
+  - intros; eapply (sd_final_determ (RelocProgSemantics2.semantics_determinate p rs)); eauto.
+Qed.
+
+Theorem reloc_prog_receptive p rs:
+  receptive (semantics p rs).
+Proof.
+  destruct (RelocProgSemantics2.reloc_prog_receptive p rs).
+  split; auto.
+Qed.
+
+End WITHEXTERNALCALLS.
